Functions
Signed-off-by: zeramorphic <zeramorphic@proton.me>

SetTheory/Function.lean
@@ -2,11 +2,108 @@ import SetTheory.Relation
 
 namespace SetTheory
 
-variable [Zermelo V] {r x y z : V}
+variable [Zermelo V] {r x y z a b c : V}
 
 /-- A set `f` is a function if all its elements are ordered pairs, and any two pairs of the form
 `⟨x, s⟩, ⟨x, t⟩` in `f` have `s = t`. -/
 structure IsFunction (f : V) extends IsRelation f : Prop where
-  eq : ∀ x s t, opair x s ∈ f → opair s t ∈ f → s = t
+  eq : ∀ x s t, opair x s ∈ f → opair x t ∈ f → s = t
+
+/-- A *function* `x ⟶ y` is a relation `f` with domain equal to `x` and range contained in `y`,
+such that if `(a, b), (a, c) ∈ f`, we have `b = c`. -/
+structure Function (x y : V) where
+  graph : V
+  isFunction : IsFunction graph
+  dom_eq : dom graph = x
+  ran_subset : ran graph ⊆ y
+
+infixr:10 " ⟶ " => Function
+
+theorem mem_of_mem_dom (f : a ⟶ b) (hx : x ∈ dom f.graph) : x ∈ a :=
+  by rwa [← f.dom_eq]
+
+theorem mem_dom_of_mem (f : a ⟶ b) (hx : x ∈ a) : x ∈ dom f.graph :=
+  by rwa [f.dom_eq]
+
+def apply (f x : V) : V := ⋃ image f {x}
+
+instance : CoeFun V (fun _ => V → V) where
+  coe := apply
+
+instance : CoeFun (a ⟶ b) (fun _ => V → V) where
+  coe f := f.graph
+
+theorem mem_apply_iff {f : V} : y ∈ f x ↔ ∃ z, opair x z ∈ f ∧ y ∈ z := by
+  unfold apply
+  simp [mem_image_iff]
+
+theorem eq_of_opair_mem_graph (f : a ⟶ b) (h : opair x y ∈ f.graph) : y = f x := by
+  ext z
+  rw [mem_apply_iff]
+  constructor
+  · intro h'
+    exact ⟨_, h, h'⟩
+  · intro ⟨t, ht, ht'⟩
+    cases f.isFunction.eq x y t h ht
+    exact ht'
+
+theorem opair_mem_graph (f : a ⟶ b) (h : x ∈ a) : opair x (f x) ∈ f.graph := by
+  have := mem_dom_of_mem f h
+  rw [mem_dom_iff] at this
+  rcases this with ⟨y, hy⟩
+  cases eq_of_opair_mem_graph f hy
+  exact hy
+
+theorem opair_mem_graph_iff (f : a ⟶ b) (h : x ∈ a) : opair x y ∈ f.graph ↔ y = f x := by
+  constructor
+  · exact eq_of_opair_mem_graph f
+  · rintro rfl
+    exact opair_mem_graph f h
+
+/-- **Function extensionality**. Two functions are equal if they agree at all inputs in their domains. -/
+@[ext]
+theorem Function.ext {f g : a ⟶ b} (h : ∀ x ∈ a, f x = g x) : f = g := by
+  suffices f.graph = g.graph from by
+    cases f
+    cases this
+    rfl
+  ext x
+  constructor
+  · intro hx
+    obtain ⟨x, y, rfl⟩ := f.isFunction.isOPair x hx
+    have : x ∈ a := by
+      refine mem_of_mem_dom f ?_
+      rw [mem_dom_iff]
+      exact ⟨y, hx⟩
+    rw [opair_mem_graph_iff _ this] at hx ⊢
+    rw [hx]
+    exact h _ this
+  · intro hx
+    obtain ⟨x, y, rfl⟩ := g.isFunction.isOPair x hx
+    have : x ∈ a := by
+      refine mem_of_mem_dom g ?_
+      rw [mem_dom_iff]
+      exact ⟨y, hx⟩
+    rw [opair_mem_graph_iff _ this] at hx ⊢
+    rw [hx]
+    exact (h _ this).symm
+
+def comp (g : b ⟶ c) (f : a ⟶ b) : a ⟶ c where
+  graph := rcomp g.graph f.graph
+  isFunction := {
+    rcomp_isRelation f.isFunction.toIsRelation with
+    eq := by
+      intro x s t hs ht
+      rw [opair_mem_rcomp_iff] at hs ht
+      obtain ⟨u, hgu, hfu⟩ := hs
+      obtain ⟨v, hgv, hfv⟩ := ht
+      cases f.isFunction.eq x u v hfu hfv
+      exact g.isFunction.eq u s t hgu hgv
+  }
+  dom_eq := by
+    rw [dom_rcomp, f.dom_eq]
+    rw [g.dom_eq]
+    exact f.ran_subset
+  ran_subset := subset_trans ran_rcomp g.ran_subset
 
 end SetTheory
